type/3_19.v
@@ -1,0 +1,1007 @@
+From SST Require Export type.global type.local type.isomorphism type.projection.
+Require Import List String Datatypes ZArith Relations PeanoNat.
+Open Scope list_scope.
+From Paco Require Import paco pacotac.
+Require Import Setoid Morphisms Coq.Program.Basics.
+Require Import Coq.Init.Datatypes.
+
+Lemma step_mon : monotone5 gttstep.
+Admitted.
+
+Lemma gttT_mon : monotone2 gttT.
+Admitted.
+
+Lemma merge_less_recv : forall p LQ o1 ys1,
+    isMerge (ltt_recv p LQ) (o1 :: ys1) -> exists LQ0, isMerge (ltt_recv p LQ0) ys1.
+Admitted.
+
+Lemma merge_less_send : forall q LP o2 ys0,
+    isMerge (ltt_send q LP) (o2 :: ys0) -> exists LP0, isMerge (ltt_send q LP0) ys0.
+Admitted.
+
+Lemma _a_26 : forall T xt xs,
+  isMerge T (Some xt :: xs) -> subtypeC T xt.
+Admitted.
+
+Lemma _a_26s : forall T lis,
+  isMerge T lis -> List.Forall (fun u => u = None \/ (exists T', u = Some T' /\ subtypeC T T')) lis.
+Admitted.
+
+Lemma triv_merge : forall T T', isMerge T (Some T' :: nil) -> T = T'.
+Admitted.
+
+Lemma triv_merge2 : forall T xs, isMerge T xs -> isMerge T (None :: xs).
+Admitted.
+
+Lemma merge_onth_recv : forall n p LQ ys1 gqT,
+      isMerge (ltt_recv p LQ) ys1 ->
+      onth n ys1 = Some gqT -> 
+      exists LQ', gqT = ltt_recv p LQ'.
+Admitted.
+
+Lemma merge_onth_send : forall n q LP ys0 gpT,
+      isMerge (ltt_send q LP) ys0 ->
+      onth n ys0 = Some gpT ->
+      exists LP', gpT = (ltt_send q LP').
+Admitted.
+
+
+Lemma more_merge_sub: forall T T' o0 ys0,
+          isMerge T ys0 ->
+          isMerge T' (o0 :: ys0) ->
+          subtypeC T' T.
+Admitted.
+
+Lemma merge_label_recv : forall Mp LQ' LQ0' T k l p,
+          isMerge (ltt_recv p LQ') Mp ->
+          onth k Mp = Some (ltt_recv p LQ0') ->
+          onth l LQ0' = Some T ->
+          exists T', onth l LQ' = Some T'.
+Admitted.
+
+Lemma merge_label_send : forall Mq LP' LP0' T k l q,
+          isMerge (ltt_send q LP') Mq ->
+          onth k Mq = Some (ltt_send q LP0') ->
+          onth l LP0' = Some T ->
+          exists T', onth l LP' = Some T'. 
+Admitted.
+
+Lemma in_some_implies_onth {A} : forall (x : A) xs,
+    In (Some x) xs -> exists n, onth n xs = Some x.
+Proof.
+  intros. revert H. revert x. 
+  induction xs; intros; try easy.
+  simpl in *. destruct H. exists 0. easy.
+  specialize(IHxs x H). destruct IHxs. exists (Nat.succ x0). easy.
+Qed.
+
+Lemma proj_inv_lis : forall Gl p q l s s' ys ctxG T T' SI LP LQ G',
+    (ishParts p Gl -> False) ->
+    (ishParts q Gl -> False) ->
+    Forall
+       (fun u : option gtt =>
+        u = None \/
+        (exists (g : gtt) (lsg : list (option (sort * gtt))),
+           u = Some g /\
+           g = gtt_send p q lsg /\
+           (exists (s' : sort) (Gjk : gtt) (Tp Tq : ltt),
+              onth l lsg = Some (s', Gjk) /\
+              projectionC Gjk p Tp /\ T = Tp /\ projectionC Gjk q Tq /\ T' = Tq) /\
+           Forall2
+             (fun (u0 : option (sort * gtt)) (v : option sort) =>
+              u0 = None /\ v = None \/
+              (exists (s : sort) (g' : gtt), u0 = Some (s, g') /\ v = Some s)) lsg SI))
+       ctxG ->
+    typ_gtth ctxG Gl (gtt_send s s' ys) ->
+    projectionC (gtt_send s s' ys) p (ltt_send q LP) -> 
+    projectionC (gtt_send s s' ys) q (ltt_recv p LQ) -> 
+    gttstepC (gtt_send s s' ys) G' p q l ->
+    (s = p /\ s' = q /\ exists Gk, onth l ys = Some Gk) \/
+    (s <> p /\ s' <> q /\ List.Forall (fun u => u = None \/ 
+        (exists s g LP' LQ' T T', u = Some(s, g) /\ projectionC g p (ltt_send q LP') /\ projectionC g q (ltt_recv p LQ') /\ 
+          onth l LP' = Some T /\ onth l LQ' = Some T')) ys).
+Proof.
+  intro Gl. induction Gl using gtth_ind_ref; intros; try easy.
+  - inversion H2. subst.
+    specialize(some_onth_implies_In n ctxG (gtt_send s s' ys) H8); intros.
+    specialize(Forall_forall (fun u : option gtt =>
+            u = None \/
+            (exists (g : gtt) (lsg : list (option (sort * gtt))),
+               u = Some g /\
+               g = gtt_send p q lsg /\
+               (exists (s' : sort) (Gjk : gtt) (Tp Tq : ltt),
+                  onth l lsg = Some (s', Gjk) /\
+                  projectionC Gjk p Tp /\
+                  T = Tp /\ projectionC Gjk q Tq /\ T' = Tq) /\
+               Forall2
+                 (fun (u0 : option (sort * gtt)) (v : option sort) =>
+                  u0 = None /\ v = None \/
+                  (exists (s : sort) (g' : gtt),
+                     u0 = Some (s, g') /\ v = Some s)) lsg SI)) ctxG); intros. destruct H7.
+    specialize(H7 H1). clear H1 H9. specialize(H7 (Some (gtt_send s s' ys)) H6).
+    destruct H7; try easy. destruct H1. destruct H1. destruct H1. destruct H7. destruct H9.
+    destruct H9. destruct H9. destruct H9. destruct H9. destruct H9. destruct H11. destruct H12. destruct H13. destruct H14. 
+    subst. inversion H1. subst.
+    left. split; try easy. split; try easy. exists (x1, x2). easy.
+  - inversion H3. subst. right. 
+    pinversion H4; try easy. subst.
+    assert False. apply H0. constructor. easy.
+    subst. clear H14. split; try easy. 
+    pinversion H5; try easy. subst. split; try easy. 
+    rename p0 into p. rename q0 into q. clear H20.
+    pinversion H6; try easy. subst.
+    apply Forall_forall; intros; try easy. destruct x.
+    - right. destruct p0. clear H14 H16 H17.
+      specialize(in_some_implies_onth (s0, g) ys H7); intros. destruct H8. rename x into n.
+      assert(exists t t' g' g'', onth n ys1 = Some t /\ projectionC g q t /\ onth n ys0 = Some t' /\ projectionC g p t' /\ onth n xs = Some (s0, g') /\ typ_gtth ctxG g' g /\ onth n ys2 = Some (s0, g'') /\ gttstepC g g'' p q l /\ 
+              (forall (p q : string) (l : fin) (s0 s' : string)
+                 (ys : list (option (sort * gtt))) (ctxG : list (option gtt)) 
+                 (T T' : ltt) (SI : list (option sort)) (LP LQ : list (option (sort * ltt)))
+                 (G' : gtt),
+               (ishParts p g' -> False) ->
+               (ishParts q g' -> False) ->
+               Forall
+                 (fun u0 : option gtt =>
+                  u0 = None \/
+                  (exists (g0 : gtt) (lsg : list (option (sort * gtt))),
+                     u0 = Some g0 /\
+                     g0 = gtt_send p q lsg /\
+                     (exists (s'0 : sort) (Gjk : gtt) (Tp Tq : ltt),
+                        onth l lsg = Some (s'0, Gjk) /\
+                        projectionC Gjk p Tp /\ T = Tp /\ projectionC Gjk q Tq /\ T' = Tq) /\
+                     Forall2
+                       (fun (u1 : option (sort * gtt)) (v : option sort) =>
+                        u1 = None /\ v = None \/
+                        (exists (s1 : sort) (g' : gtt), u1 = Some (s1, g') /\ v = Some s1))
+                       lsg SI)) ctxG ->
+               typ_gtth ctxG g' (gtt_send s0 s' ys) ->
+               projectionC (gtt_send s0 s' ys) p (ltt_send q LP) ->
+               projectionC (gtt_send s0 s' ys) q (ltt_recv p LQ) ->
+               gttstepC (gtt_send s0 s' ys) G' p q l ->
+               s0 = p /\ s' = q /\ (exists Gk : sort * gtt, onth l ys = Some Gk) \/
+               s0 <> p /\
+               s' <> q /\
+               Forall
+                 (fun u0 : option (sort * gtt) =>
+                  u0 = None \/
+                  (exists
+                     (s1 : sort) (g0 : gtt) (LP' LQ' : list (option (sort * ltt))) 
+                   (T0 T'0 : sort * ltt),
+                     u0 = Some (s1, g0) /\
+                     projectionC g0 p (ltt_send q LP') /\
+                     projectionC g0 q (ltt_recv p LQ') /\
+                     onth l LP' = Some T0 /\ onth l LQ' = Some T'0)) ys)
+      ).
+      {
+        clear H7 H28 H27 H26 H25 H22 H21 H20 H24 H19 H13 H12 H11 H6 H5 H4 H3 H1 H0 H10.
+        clear H2. revert H8 H34 H33 H23 H18 H15 H. revert xs p q l s s' ctxG T T' SI LP LQ ys2 ys0 ys1 s0 g n.
+        induction ys; intros; try easy. destruct n; try easy. 
+        destruct ys2; try easy. destruct ys1; try easy. destruct xs; try easy. destruct ys0; try easy.
+        inversion H34. subst. clear H34. inversion H. subst. clear H.
+        inversion H33. subst. clear H33. inversion H23. subst. clear H23.
+        inversion H18. subst. clear H18. inversion H15. subst. clear H15.
+        
+        destruct n.
+        - simpl in *. subst.
+          destruct H3; try easy. destruct H. destruct H. destruct H. destruct H. destruct H0.
+          inversion H. subst. clear H.
+          clear H16 H13 H11 H6 H4 H5 IHys.
+          destruct H1; try easy. destruct H. destruct H. destruct H. destruct H0. 
+          inversion H. subst. clear H.
+          destruct H9; try easy. destruct H. destruct H. destruct H. destruct H. destruct H4. 
+          inversion H. subst. clear H.
+          destruct H10; try easy. destruct H. destruct H. destruct H. destruct H. destruct H4.
+          inversion H. subst. clear H.
+          destruct H12; try easy. destruct H. destruct H. destruct H. destruct H. destruct H4.
+          inversion H4. subst. clear H4.
+          destruct H2; try easy. destruct H. destruct H. destruct H. inversion H. subst.
+          exists x4. exists x5. exists x3. exists x1. pclearbot. easy.
+        - simpl in *.
+          apply IHys; try easy.
+      }
+      clear H34 H33 H23 H18 H15 H. clear H11 H12 H13.
+      destruct H9. destruct H. destruct H. destruct H. destruct H. destruct H9. destruct H11.
+      destruct H12. destruct H13. destruct H14. destruct H15. destruct H16.
+      rename x0 into gpT. rename x1 into g'. rename x2 into g''. rename x into gqT.
+      destruct g; try easy. pinversion H16; try easy. apply step_mon.
+      specialize(H17 p q l s1 s2 l0 ctxG T T' SI).
+      specialize(merge_onth_send n q LP ys0 gpT H19 H11); intros. destruct H18. subst.
+      specialize(merge_onth_recv n p LQ ys1 gqT H24 H); intros. destruct H18. subst.
+      rename x0 into LQ'. rename x into LP'.
+      specialize(H17 LP' LQ' g''). 
+      exists s0. exists (gtt_send s1 s2 l0). exists LP'. exists LQ'.
+      assert (ishParts p g' -> False).
+      {
+        intros. apply H0.
+        - case_eq (eqb p s); intros.
+          assert (p = s). apply eqb_eq; try easy. subst. apply ha_sendp.
+        - case_eq (eqb p s'); intros.
+          assert (p = s'). apply eqb_eq; try easy. subst. apply ha_sendq.
+        - assert (p <> s). apply eqb_neq; try easy. 
+          assert (p <> s'). apply eqb_neq; try easy.
+          apply ha_sendr with (n := n) (s := s0) (g := g'); try easy. 
+      }
+      assert (ishParts q g' -> False).
+      {
+        intros. apply H1.
+        - case_eq (eqb q s); intros.
+          assert (q = s). apply eqb_eq; try easy. subst. apply ha_sendp.
+        - case_eq (eqb q s'); intros.
+          assert (q = s'). apply eqb_eq; try easy. subst. apply ha_sendq.
+        - assert (q <> s). apply eqb_neq; try easy. 
+          assert (q <> s'). apply eqb_neq; try easy.
+          apply ha_sendr with (n := n) (s := s0) (g := g'); try easy.
+      }
+      assert (s1 = p /\ s2 = q /\ (exists Gk : sort * gtt, onth l l0 = Some Gk) \/
+      s1 <> p /\
+      s2 <> q /\
+      Forall
+        (fun u0 : option (sort * gtt) =>
+         u0 = None \/
+         (exists (s1 : sort) (g0 : gtt) (LP' LQ' : list (option (sort * ltt))) 
+          (T0 T'0 : sort * ltt),
+            u0 = Some (s1, g0) /\
+            projectionC g0 p (ltt_send q LP') /\
+            projectionC g0 q (ltt_recv p LQ') /\ onth l LP' = Some T0 /\ onth l LQ' = Some T'0)) l0).
+      {
+        apply H17; try easy.
+      }
+      
+      destruct H29.
+      - destruct H29. destruct H30. destruct H31. subst. clear H17 H2.
+        pinversion H9; try easy. subst. pinversion H12; try easy. subst.
+        destruct x.
+        assert(exists T0 T'0, onth l LP' = Some T0 /\ onth l LQ' = Some T'0).
+        {
+          clear H0 H1 H3 H4 H5 H6 H10 H19 H24 H20 H21 H22 H25 H26 H27 H28 H7.
+          clear H8 H9 H12 H11 H13 H14 H15 H16 H18 H23 H17 H34 H30 H.
+          clear xs s s' ys ctxG T T' s0 LP LQ ys2 ys0 ys1 s0 g' g''. clear SI n.
+          revert H31 H32 H36.
+          revert p q l LQ' LP' s1 g. induction l0; intros; try easy.
+          destruct l; try easy.
+          destruct LQ'; try easy. destruct LP'; try easy. 
+          inversion H32. subst. inversion H36. subst. clear H32 H36.
+          destruct l. simpl in *. subst.
+          destruct H2; try easy. destruct H. destruct H. destruct H. destruct H. destruct H0.
+          inversion H. subst. clear H.
+          destruct H3; try easy. destruct H. destruct H. destruct H. destruct H. destruct H0.
+          inversion H. subst. clear H.
+          exists (x2, x4). exists (x2, x1). split; try easy.
+          specialize(IHl0 p q l LQ' LP' s1 g). apply IHl0; try easy.
+        }
+        destruct H2. destruct H2. exists x. exists x0.
+        split. easy. split. pfold. easy. split. pfold. easy. easy.
+        apply proj_mon. apply proj_mon. 
+      - destruct H29. destruct H30.
+        inversion H14. subst.
+        - clear H31 H17 H18 H23 H16 H15 H13 H14 H11 H12 H H9 H8 H7 H28 H27 H26 H25 H22 H21 H20 H24 H19.
+          clear H10 H6 H5 H4 H3 H1 H0.
+          assert False.
+          clear LQ' LP' g'' n s0 ys0 ys1 ys2. clear LP LQ ys s s'. clear xs.
+          revert H32 H30 H29 H2. revert p q l T T' SI s1 s2 l0 n0.
+          induction ctxG; intros; try easy. destruct n0; try easy.
+          inversion H2. subst. clear H2. 
+          destruct n0. simpl in H32.
+          - subst. destruct H1; try easy. destruct H. destruct H. destruct H.
+            destruct H0. inversion H. subst. inversion H4. subst. easy.
+          - specialize(IHctxG p q l T T' SI s1 s2 l0 n0). apply IHctxG; try easy.
+            easy.
+        - subst.
+          assert (exists k s4 g2 LP' LQ' T0 T'0, onth k l0 = Some(s4, g2) /\ projectionC g2 p (ltt_send q LP') /\ projectionC g2 q (ltt_recv p LQ') /\ onth l LP' = Some T0 /\ onth l LQ' = Some T'0).
+          {
+            clear H30 H29 H17 H18 H23 H16 H15 H13 H14 H11 H12 H9 H8 H7 H28 H27 H26 H25 H22 H21 H.
+            clear H20 H24 H19 H10 H6 H5 H4 H3 H2 H1 H0. revert H38 H36 H31.
+            revert xs p q l s s' ys ctxG T T' SI LP LQ ys2 ys0 ys1 s0 s1 s2 l0 n g'' LQ' LP'.
+            induction xs0; try easy.
+            intros.
+            destruct l0; try easy. inversion H38. subst. inversion H31. subst. clear H31 H38.
+            specialize(SList_f a xs0 H36); intros. destruct H.
+            assert (exists (k : fin) (s4 : sort) (g2 : gtt) (LP' LQ'0 : list (option (sort * ltt))) 
+        (T0 T'0 : sort * ltt),
+          onth k l0 = Some (s4, g2) /\
+          projectionC g2 p (ltt_send q LP') /\
+          projectionC g2 q (ltt_recv p LQ'0) /\ onth l LP' = Some T0 /\ onth l LQ'0 = Some T'0).
+            {
+              apply IHxs0 with (p := p) (q := q) (l0 := l0) (ctxG := ctxG); try easy.
+            }
+            destruct H0. exists (Nat.succ x). easy.
+            
+            destruct H. destruct H0. subst. destruct l0; try easy.
+            destruct H2; try easy. destruct H. destruct H. destruct H. destruct H. destruct H0.
+            inversion H. subst.
+            destruct H1; try easy. destruct H0. destruct H0. destruct H0. destruct H0. destruct H0.
+            destruct H0. destruct H0. destruct H1. destruct H5. destruct H6. inversion H0. subst.
+            exists 0. exists x. exists x3. exists x4. exists x5. exists x6. exists x7. easy.
+          }
+          destruct H32. destruct H32. destruct H32. destruct H32. destruct H32. 
+          destruct H32. destruct H32. destruct H32. destruct H33. destruct H34. 
+          destruct H35. rename x2 into LP0'. rename x3 into LQ0'. clear H31.
+          
+          pinversion H9; try easy. subst.
+          pinversion H12; try easy. subst. 
+          clear H44 H50.
+          clear H38 H36 H30 H29 H17 H18 H23 H16 H15 H13 H14 H11 H8 H7 H28 H27.
+          clear H26 H25 H22 H21 H20 H24 H19 H10 H6 H5 H4 H3 H2 H1 H0 H.
+          assert (exists t t', onth x ys3 = Some t /\ projectionC x1 q t /\ onth x ys4 = Some t' /\ projectionC x1 p t').
+          {
+              clear H49 H46 H45 H43 H42 H41 H34 H33 H48 H54 H12 H9 .
+              clear xs s s' ys T T' SI LP LQ ys2 ys0 ys1. clear xs0 g''. clear n. clear ctxG.
+              revert H32 H35 H37 H47 H53. 
+              revert p q l s0 s1 s2 LQ' LP' x x0 x1 LP0' LQ0' x4 x5 ys3 ys4.
+              induction l0; intros; try easy.
+              - destruct x; try easy.
+              - destruct ys3; try easy. destruct ys4; try easy.
+              inversion H47. subst. inversion H53. subst. clear H47 H53.
+              destruct x.
+              - simpl in H32. subst. destruct H2; try easy. destruct H. destruct H. destruct H.
+                destruct H. destruct H0. inversion H. subst.
+                destruct H3; try easy. destruct H0. destruct H0. destruct H0. destruct H0. destruct H2.
+                inversion H0. subst.
+                exists x3. exists x6. pclearbot. easy.
+              - simpl. apply IHl0 with (l := l) (x0 := x0) (x4 := x4) (x5 := x5) (LP0' := LP0') (LQ0' := LQ0'); try easy.
+          }
+          destruct H. destruct H. destruct H. destruct H0. destruct H1.
+          specialize(proj_inj H2 H33); intros. subst.
+          specialize(proj_inj H0 H34); intros. subst.
+          rename ys3 into Mp. rename ys4 into Mq. rename x into k.
+          specialize(merge_label_send Mq LP' LP0' x4 k l q H54 H1 H35); intros.
+          destruct H3. 
+          specialize(merge_label_recv Mp LQ' LQ0' x5 k l p H48 H H37); intros.
+          destruct H4.
+          exists x. exists x2. pclearbot. split. easy. split. pfold. easy. split. pfold. easy. easy.
+        apply proj_mon.
+        apply proj_mon.
+    - left. easy.
+    apply step_mon. apply proj_mon. apply proj_mon.
+Qed.
+
+Lemma _3_19_1_helper : forall p q l G G' LP LQ S T S' T',
+  wfgC G -> 
+  projectionC G p (ltt_send q LP) ->
+  onth l LP = Some(S, T) ->
+  projectionC G q (ltt_recv p LQ) -> 
+  onth l LQ = Some(S', T') ->
+  gttstepC G G' p q l -> 
+  projectionC G' p T.
+Proof.
+  intros.
+  specialize(_a_29_s G p q LP LQ S T S' T' l H H0 H1 H2 H3); intros.
+  destruct H5. rename x into Gl. clear H.
+  revert H0 H1 H2 H3 H4 H5. revert p q l G G' LP LQ S S' T T'.
+  induction Gl using gtth_ind_ref; intros.
+  - destruct H5. destruct H. destruct H. destruct H. destruct H5. destruct H6. destruct H7. destruct H8. destruct H9.
+    rename x1 into Sn. rename x0 into SI. rename x into ctxG. 
+    inversion H. subst.
+    specialize(some_onth_implies_In n ctxG G H13); intros.
+    specialize(Forall_forall (fun u : option gtt =>
+        u = None \/
+        (exists (g : gtt) (lsg : list (option (sort * gtt))),
+           u = Some g /\
+           g = gtt_send p q lsg /\
+           (exists (s' : sort) (Gjk : gtt) (Tp Tq : ltt),
+              onth l lsg = Some (s', Gjk) /\
+              projectionC Gjk p Tp /\ T = Tp /\ projectionC Gjk q Tq /\ T' = Tq) /\
+           Forall2
+             (fun (u0 : option (sort * gtt)) (v : option sort) =>
+              u0 = None /\ v = None \/ (exists (s : sort) (g' : gtt), u0 = Some (s, g') /\ v = Some s))
+             lsg SI)) ctxG); intros. destruct H12.
+    specialize(H12 H7). clear H7 H14. 
+    specialize(H12 (Some G) H11). destruct H12; try easy.
+    destruct H7. destruct H7. destruct H7. destruct H12. destruct H14.
+    destruct H14. destruct H14. destruct H14. destruct H14. destruct H14. destruct H16. destruct H17. destruct H18.
+    subst. inversion H7. subst. clear H7.
+    pinversion H4; try easy. subst. specialize(eq_trans H25 H14); intros. inversion H7. subst. easy.
+    apply step_mon.
+  - rename p into s. rename q into s'. rename p0 into p. rename q0 into q.
+    destruct H5. destruct H5. destruct H5. destruct H5. destruct H6. destruct H7. destruct H8. destruct H9. destruct H10.
+    rename x into ctxG. rename x1 into Sn. rename x0 into SI. 
+    inversion H5. subst. 
+    pinversion H0; try easy. subst.
+    assert False. apply H6. constructor. easy.
+    pinversion H2; try easy. subst.
+    pinversion H4; try easy. subst. 
+    
+    specialize(proj_inv_lis (gtth_send s s' xs) p q l s s' ys ctxG T T' SI LP LQ (gtt_send s s' ys2)); intros.
+    assert (s = p /\ s' = q /\ (exists Gk : sort * gtt, onth l ys = Some Gk) \/
+      s <> p /\
+      s' <> q /\
+      Forall
+        (fun u : option (sort * gtt) =>
+         u = None \/
+         (exists (s : sort) (g : gtt) (LP' LQ' : list (option (sort * ltt))) 
+          (T T' : sort * ltt),
+            u = Some (s, g) /\
+            projectionC g p (ltt_send q LP') /\
+            projectionC g q (ltt_recv p LQ') /\ onth l LP' = Some T /\ onth l LQ' = Some T')) ys).
+    {
+      pclearbot.
+      apply H12; try easy. pfold. easy. pfold. easy. pfold. easy.
+    }
+    destruct H13; try easy. destruct H13. destruct H14.
+    clear H20 H31 H15 H16 H19 H28 H29 H30 H21 H13 H14 H12.
+        
+    assert (List.Forall (fun u => u = None \/ (exists s g, u = Some (s, g) /\ projectionC g p T)) ys2).
+    {
+      clear H5 H4 H2 H0 H17.
+      
+    }
+    
+    
+    
+    revert H H0 H1 H2 H3 H4 H5. revert s s' p q l G G' LP LQ S S' T T'.
+    - induction xs; intros; try easy.
+      destruct H5. destruct H5. destruct H5. destruct H5. inversion H5; try easy.
+    - destruct H5. destruct H5. destruct H5. destruct H5. destruct H6. destruct H7. destruct H8. destruct H9. destruct H10. inversion H5. subst.
+      specialize(IHxs s s' p q l); intros. rename x1 into Sn. rename x0 into SI. rename x into ctxG.
+      
+      pinversion H0; try easy.
+      - subst. assert False. apply H6. constructor. easy.
+      pinversion H2; try easy.
+      subst. clear H20 H31. 
+      pinversion H4; try easy. subst.
+      clear H28 H29 H30. 
+      
+      destruct ys; try easy. destruct ys0; try easy. destruct ys1; try easy. destruct ys2; try easy.
+      specialize(IHxs (gtt_send s s' ys) (gtt_send s s' ys2) LP LQ S S' T T').
+      
+      specialize(SList_f a xs H17); intros. clear H17.
+      destruct H12.
+      - assert (projectionC (gtt_send s s' ys2) p T).
+        {
+          apply IHxs; try easy.
+          inversion H; try easy.
+        }
+      - destruct H12. destruct H13. subst.
+        inversion H18. subst. clear H18. inversion H38. subst. clear H38.
+        inversion H39. subst. clear H39. inversion H. subst. clear H.
+        inversion H34. subst. clear H34. inversion H23. subst. clear H23.
+        destruct ys; try easy. destruct ys0; try easy. destruct ys1; try easy. destruct ys2; try easy.
+        clear H39 H38 H32 H33 H18 H29 IHxs.
+        destruct H17; try easy. destruct H. destruct H. destruct H. destruct H. destruct H12.
+        inversion H. subst. clear H.
+        destruct H30; try easy. destruct H. destruct H. destruct H. destruct H. destruct H12.
+        inversion H. subst. clear H.
+        destruct H34; try easy. destruct H. destruct H. destruct H. destruct H. destruct H12.
+        inversion H. subst. clear H.
+        destruct H14; try easy. destruct H. destruct H. destruct H. destruct H12.
+        inversion H. subst. clear H.
+        destruct H36; try easy. destruct H. destruct H. destruct H. destruct H. destruct H23. 
+        inversion H. subst. clear H.
+        destruct H28; try easy. destruct H. destruct H. destruct H.
+        inversion H. subst. clear H.
+        specialize(H23 p q l).
+        rename x2 into G. rename x4 into G'. rename x3 into Gl.
+        specialize(triv_merge (ltt_send q LP) x5 H24); intros. subst.
+        specialize(triv_merge (ltt_recv p LQ) x6 H35); intros. subst.
+        specialize(H23 G G' LP LQ S S' T T').
+        assert (projectionC G' p T).
+        {
+          pclearbot.
+          apply H23; try easy.
+          destruct H17; try easy.
+          exists ctxG. exists SI. exists Sn. 
+          split. easy.
+          split; intros.
+          - apply H6. 
+            - case_eq (eqb p s); intros.
+              assert (p = s). apply eqb_eq; try easy. subst. apply ha_sendp.
+            - case_eq (eqb p s'); intros.
+              assert (p = s'). apply eqb_eq; try easy. subst. apply ha_sendq.
+            - assert (p <> s). apply eqb_neq; try easy. 
+              assert (p <> s'). apply eqb_neq; try easy.
+              apply ha_sendr with (n := 0) (s := x) (g := Gl); try easy.
+          split; intros.
+          - apply H7.
+            - case_eq (eqb q s); intros.
+              assert (q = s). apply eqb_eq; try easy. subst. apply ha_sendp.
+            - case_eq (eqb q s'); intros.
+              assert (q = s'). apply eqb_eq; try easy. subst. apply ha_sendq.
+            - assert (q <> s). apply eqb_neq; try easy. 
+              assert (q <> s'). apply eqb_neq; try easy.
+              apply ha_sendr with (n := 0) (s := x) (g := Gl); try easy.
+          split; try easy.
+        }
+        clear H23 H8.
+        destruct T.
+        - pinversion H; try easy. subst.
+          pfold. constructor; try easy. intros. apply H8.
+          - admit. (* isParts in continuation *)
+          apply proj_mon.
+        - pfold.
+          apply proj_cont with (ys := (Some (ltt_recv s0 l0) :: nil)); try easy.
+          constructor; try easy. right. exists x. exists G'. exists (ltt_recv s0 l0). 
+          split. easy. split. easy. left. easy.
+        - pfold. 
+          apply proj_cont with (ys := (Some (ltt_send s0 l0) :: nil)); try easy. 
+          constructor; try easy. right. exists x. exists G'. exists (ltt_send s0 l0).
+          split. easy. split. easy. left. easy.
+    apply step_mon.
+    apply proj_mon.
+    apply proj_mon.
+
+Lemma _3_19_1 : forall p q l G G' LP LQ S T S' T' xs,
+  wfgC G ->
+  projectionC G p (ltt_send q LP) ->
+  subtypeC (ltt_send q (extendLis l (Datatypes.Some (S,T)))) (ltt_send q LP) ->
+  projectionC G q (ltt_recv p LQ) ->
+  onth l xs = Some (S', T') ->
+  subtypeC (ltt_recv p xs) (ltt_recv p LQ) ->
+  gttstepC G G' p q l ->
+  exists L, 
+  projectionC G' p L /\ subtypeC T L. 
+Proof.
+  
+ 
+    - specialize(IHxs s s' p q l).
+      inversion H. subst. clear H.
+      assert(forall (G G' : gtt) (S : sort) (T : ltt) 
+         (S' : sort) (T' : ltt) (xs0 : list (option (sort * ltt))) (LP LQ : list (option (sort * ltt))),
+      wfgC G ->
+      projectionC G p (ltt_send q LP) ->
+      subtypeC (ltt_send q (extendLis l (Some (S, T)))) (ltt_send q LP) ->
+      projectionC G q (ltt_recv p LQ) ->
+      onth l xs0 = Some (S', T') ->
+      subtypeC (ltt_recv p xs0) (ltt_recv p LQ) ->
+      gttstepC G G' p q l ->
+      (exists (ctxG : list (option gtt)) (SI : list (option sort)) (Sn : sort),
+         typ_gtth ctxG (gtth_send s s' xs) G /\
+         (ishParts p (gtth_send s s' xs) -> False) /\
+         (ishParts q (gtth_send s s' xs) -> False) /\
+         Forall
+              (fun u : option gtt =>
+               u = None \/
+               (exists (g0 : gtt) (lsg : list (option (sort * gtt))),
+                  u = Some g0 /\
+                  g0 = gtt_send p q lsg /\
+                  (exists (s' : sort) (Gjk : gtt) (Tp Tq : ltt),
+                     onth l lsg = Some (s', Gjk) /\
+                     projectionC Gjk p Tp /\ subtypeC T Tp /\ projectionC Gjk q Tq /\ subtypeC T' Tq) /\
+                  Forall2
+                    (fun (u0 : option (sort * gtt)) (v : option sort) =>
+                     u0 = None /\ v = None \/
+                     (exists (s0 : sort) (g' : gtt), u0 = Some (s0, g') /\ v = Some s0)) lsg SI)) ctxG /\
+           onth l SI = Some Sn /\ subsort S Sn /\ subsort Sn S') ->
+        exists L : ltt, projectionC G' p L /\ subtypeC T L).
+      {
+        intros.
+        specialize(IHxs G0 G'0 LP0 LQ0 S0 T0 S'0 T'0 xs1). apply IHxs; try easy.
+      }
+      clear IHxs. rename H into IHxs. clear H11.
+      
+      destruct H7. destruct H. destruct H. destruct H. destruct H7. destruct H8. destruct H9. destruct H11. destruct H12.
+     
+      destruct ys0; try easy. destruct ys1; try easy. destruct ys2; try easy.
+      
+      specialize(SList_f a xs H19); intros. destruct H14.
+      
+      specialize(IHxs (gtt_send s s' ys) (gtt_send s s' ys2) S T S' T' xs0).
+      assert(forall LP LQ : list (option (sort * ltt)),
+       wfgC (gtt_send s s' ys) ->
+       projectionC (gtt_send s s' ys) p (ltt_send q LP) ->
+       subtypeC (ltt_send q (extendLis l (Some (S, T)))) (ltt_send q LP) ->
+       projectionC (gtt_send s s' ys) q (ltt_recv p LQ) ->
+       subtypeC (ltt_recv p xs0) (ltt_recv p LQ) ->
+       exists L : ltt, projectionC (gtt_send s s' ys2) p L /\ subtypeC T L).
+      {
+        intros. specialize(IHxs LP0 LQ0). apply IHxs; try easy.
+        - inversion H41. inversion H42. subst. pfold. constructor; try easy.
+          admit. (* removing 1 thing from wfgC *)
+        exists ctxG. exists SI. exists Sn.
+        - split. constructor; try easy.
+        - split; intros. apply H7. inversion H31.
+          apply ha_sendp. apply ha_sendq. 
+          apply ha_sendr with (n := Nat.succ n) (s := s0) (g := g); intros; try easy.
+        - split; intros. apply H8. inversion H31.
+          apply ha_sendp. apply ha_sendq. 
+          apply ha_sendr with (n := Nat.succ n) (s := s0) (g := g); intros; try easy.
+        - split; try easy.
+      }
+      clear IHxs. rename H15 into IHxs.
+      specialize(merge_less_recv p LQ o1 ys1 H38); intros. destruct H15.
+      specialize(merge_less_send q LP o0 ys0 H27); intros. destruct H16.
+      rename x into LQ'. rename x0 into LP'.
+      specialize(IHxs LP' LQ'); intros.
+      assert (exists L : ltt, projectionC (gtt_send s s' ys2) p L /\ subtypeC T L). 
+      {
+        apply IHxs; try easy. clear IHxs.
+        - admit. (* removing 1 thing from wfgC *)
+        - pfold. 
+          apply proj_cont with (ys := ys0); try easy. inversion H26. subst. easy.
+          apply stTrans with (l2 := (ltt_send q LP)); try easy.
+          apply more_merge_sub with (o0 := o0) (ys0 := ys0); try easy.
+        - pfold.
+          apply proj_cont with (ys := ys1); try easy. inversion H37. subst. easy.
+          apply stTrans with (l2 := (ltt_recv p LQ)); try easy.
+          apply more_merge_sub with (o0 := o1) (ys0 := ys1); try easy.
+      }
+      destruct H18. rename x into Lys. destruct H18.
+      
+      inversion H41. subst. clear H41. inversion H37. subst. clear H37.
+      inversion H42. subst. clear H42. inversion H26. subst. clear H26.
+      clear IHxs.
+      
+      destruct H10. subst.
+      - destruct H17; try easy. destruct H10. subst.
+        destruct H37. destruct H36. destruct H39. destruct H22. destruct H17. destruct H26. subst.
+        exists Lys. split; try easy.
+        pfold. 
+        pinversion H18; try easy. subst. (* participant pf, use H33 *)
+        admit.
+        subst. apply proj_cont with (ys := None :: ys3); try easy. constructor; try easy.
+        left. easy.
+        apply triv_merge2; try easy.
+        apply proj_mon.
+        destruct H26. destruct H26. destruct H26. destruct H26; try easy.
+        destruct H22. destruct H22. destruct H22. destruct H22. easy.
+        destruct H17. destruct H17. destruct H17. destruct H17. easy.
+        destruct H10. destruct H10. destruct H10. destruct H10. easy.
+        
+      - destruct H10. destruct H10. destruct H10. subst.
+        destruct H17; try easy. destruct H10. destruct H10. destruct H10. destruct H10. destruct H17.
+        inversion H10. subst. clear H10.
+        destruct H32; try easy. destruct H10. destruct H10. destruct H10. destruct H17.
+        inversion H10. subst. clear H10.
+        destruct H37; try easy. destruct H10. destruct H10. destruct H10. destruct H10. destruct H32.
+        inversion H10. subst. clear H10.
+        destruct H36; try easy. destruct H10. destruct H10. destruct H10. destruct H10. destruct H32.
+        inversion H10. subst. clear H10.
+        destruct H39; try easy. destruct H10. destruct H10. destruct H10. destruct H10. destruct H32.
+        inversion H10. subst. clear H10.
+        rename x2 into Gl. rename x3 into G. rename x4 into G'.
+        specialize(H22 p q l G G').
+        specialize(_a_29_part_helper_recv 0 (Some x5 :: ys1) x5 p LQ (eq_refl (Some x5)) H38); intros.
+        destruct H10. subst.
+        specialize(_a_29_part_helper_send 0 (Some x6 :: ys0) x6 q LP (eq_refl (Some x6)) H27); intros.
+        destruct H10. subst.
+        
+        rename x into LQs. rename x0 into LPs.
+        specialize(H22 LPs LQs S T S' T' xs0).
+        assert (exists L : ltt, projectionC G' p L /\ subtypeC T L).
+        {
+          pclearbot.
+          apply H22; try easy.
+          - admit. (* wfgC of continuation *)
+          - specialize(_a_26 (ltt_send q LP) (ltt_send q LPs) ys0 H27); intros.
+            apply stTrans with (l2 := (ltt_send q LP)); try easy.
+          - specialize(_a_26 (ltt_recv p LQ) (ltt_recv p LQs) ys1 H38); intros.
+            apply stTrans with (l2 := (ltt_recv p LQ)); try easy.
+          - destruct H35; try easy.
+          - exists ctxG. exists SI. exists Sn. 
+          split. easy.
+          - split. intros. apply H7; try easy.
+            - case_eq (eqb p s); intros.
+              assert (p = s). apply eqb_eq; try easy. subst. apply ha_sendp.
+            - case_eq (eqb p s'); intros.
+              assert (p = s'). apply eqb_eq; try easy. subst. apply ha_sendq.
+            - assert (p <> s). apply eqb_neq; try easy. 
+              assert (p <> s'). apply eqb_neq; try easy.
+              apply ha_sendr with (n := 0) (s := x1) (g := Gl); try easy.
+          - split. intros. apply H8.
+            - case_eq (eqb q s); intros.
+              assert (q = s). apply eqb_eq; try easy. subst. apply ha_sendp.
+            - case_eq (eqb q s'); intros.
+              assert (q = s'). apply eqb_eq; try easy. subst. apply ha_sendq.
+            - assert (q <> s). apply eqb_neq; try easy. 
+              assert (q <> s'). apply eqb_neq; try easy.
+              apply ha_sendr with (n := 0) (s := x1) (g := Gl); try easy.
+          - split; try easy.
+        }
+        destruct H10. destruct H10. clear H9 H22. 
+        assert (exists L, projectionC (gtt_send s s' (Some (x1, G') :: ys2)) p L). { admit. }
+        destruct H9. exists x0. rename x0 into L. split; try easy.
+        pinversion H9; try easy. subst. admit. (* doable, a bit tedious *)
+        - subst.
+        
+        
+        destruct x.
+        - exists ltt_end. split; try easy.
+          pfold. constructor; try easy.
+          admit. (* doable, a bit tedious *)
+        - 
+        
+      admit. admit.
+       
+     
+
+
+Lemma _3_19_1 : forall p q l G G' LP LQ S T S' T' xs,
+  wfgC G ->
+  projectionC G p (ltt_send q LP) ->
+  subtypeC (ltt_send q (extendLis l (Datatypes.Some (S,T)))) (ltt_send q LP) ->
+  projectionC G q (ltt_recv p LQ) ->
+  onth l xs = Some (S', T') ->
+  subtypeC (ltt_recv p xs) (ltt_recv p LQ) ->
+  gttstepC G G' p q l ->
+  exists L, 
+  projectionC G' p L /\ subtypeC T L. 
+Proof.
+  intros.
+  specialize(_a_29 G p q (ltt_send q LP) (ltt_recv p LQ) S T S' T' xs l H H0 H1 H2 H3 H4); intros.
+  destruct H6. rename x into Gl. revert H H0 H1 H2 H3 H4 H5 H6.
+  revert p q l G G' LP LQ S T S' T' xs.
+  induction Gl using gtth_ind_ref; intros; try easy.
+  - destruct H6. destruct H6. destruct H6. destruct H6. destruct H7. destruct H8. destruct H9. destruct H10. destruct H11.
+    inversion H6. subst.
+    specialize(some_onth_implies_In n x G H15); intros.
+    specialize(Forall_forall (fun u : option gtt =>
+         u = None \/
+         (exists (g : gtt) (lsg : list (option (sort * gtt))),
+            u = Some g /\
+            g = gtt_send p q lsg /\
+            (exists (s' : sort) (Gjk : gtt) (Tp Tq : ltt),
+               onth l lsg = Some (s', Gjk) /\
+               projectionC Gjk p Tp /\
+               subtypeC T Tp /\ projectionC Gjk q Tq /\ subtypeC T' Tq) /\
+            Forall2
+              (fun (u0 : option (sort * gtt)) (v : option sort) =>
+               u0 = None /\ v = None \/
+               (exists (s : sort) (g' : gtt), u0 = Some (s, g') /\ v = Some s)) lsg x0)) x); intros.
+    destruct H14. specialize(H14 H9). clear H9 H16.
+    specialize(H14 (Some G) H13). destruct H14; try easy.
+    destruct H9. destruct H9. destruct H9. destruct H14. destruct H16.
+    inversion H9. subst. 
+    destruct H16. destruct H14. destruct H14. destruct H14. destruct H14. destruct H16. destruct H18. destruct H19.
+    pinversion H5; try easy. subst.
+    specialize(eq_trans H30 H14); intros. inversion H21. subst. 
+    exists x5. split; try easy.
+    apply step_mon.
+  - rename p into s. rename q into s'. rename p0 into p. rename q0 into q.
+  
+  
+  revert H H0 H1 H2 H3 H4 H5 H6 H7.
+    
+    revert s s' p q l G G' LP LQ S T S' T' xs0.
+    induction xs; intros; try easy.
+    - destruct H7. destruct H7. destruct H7. destruct H7. destruct H8. destruct H9. 
+      inversion H7. subst. easy.
+    - specialize(IHxs s s' p q l).
+      inversion H. subst. clear H.
+      assert(forall (G G' : gtt) (S : sort) (T : ltt) 
+         (S' : sort) (T' : ltt) (xs0 : list (option (sort * ltt))) (LP LQ : list (option (sort * ltt))),
+      wfgC G ->
+      projectionC G p (ltt_send q LP) ->
+      subtypeC (ltt_send q (extendLis l (Some (S, T)))) (ltt_send q LP) ->
+      projectionC G q (ltt_recv p LQ) ->
+      onth l xs0 = Some (S', T') ->
+      subtypeC (ltt_recv p xs0) (ltt_recv p LQ) ->
+      gttstepC G G' p q l ->
+      (exists (ctxG : list (option gtt)) (SI : list (option sort)) (Sn : sort),
+         typ_gtth ctxG (gtth_send s s' xs) G /\
+         (ishParts p (gtth_send s s' xs) -> False) /\
+         (ishParts q (gtth_send s s' xs) -> False) /\
+         Forall
+              (fun u : option gtt =>
+               u = None \/
+               (exists (g0 : gtt) (lsg : list (option (sort * gtt))),
+                  u = Some g0 /\
+                  g0 = gtt_send p q lsg /\
+                  (exists (s' : sort) (Gjk : gtt) (Tp Tq : ltt),
+                     onth l lsg = Some (s', Gjk) /\
+                     projectionC Gjk p Tp /\ subtypeC T Tp /\ projectionC Gjk q Tq /\ subtypeC T' Tq) /\
+                  Forall2
+                    (fun (u0 : option (sort * gtt)) (v : option sort) =>
+                     u0 = None /\ v = None \/
+                     (exists (s0 : sort) (g' : gtt), u0 = Some (s0, g') /\ v = Some s0)) lsg SI)) ctxG /\
+           onth l SI = Some Sn /\ subsort S Sn /\ subsort Sn S') ->
+        exists L : ltt, projectionC G' p L /\ subtypeC T L).
+      {
+        intros.
+        specialize(IHxs G0 G'0 LP0 LQ0 S0 T0 S'0 T'0 xs1). apply IHxs; try easy.
+      }
+      clear IHxs. rename H into IHxs. clear H11.
+      
+      destruct H7. destruct H. destruct H. destruct H. destruct H7. destruct H8. destruct H9. destruct H11. destruct H12.
+      rename x into ctxG. rename x1 into Sn.
+      inversion H. subst. destruct ys; try easy. inversion H20. subst. clear H20.
+      
+      pinversion H1. subst. assert False. apply H7. constructor. easy.
+      pinversion H3. subst. assert False. apply H7. constructor. easy.
+      subst. clear H34 H23. rename x0 into SI.
+      pinversion H6. subst. easy. subst. clear H18 H20 H22 H31 H32 H33.
+      destruct ys0; try easy. destruct ys1; try easy. destruct ys2; try easy.
+      
+      specialize(SList_f a xs H19); intros. destruct H14.
+      
+      specialize(IHxs (gtt_send s s' ys) (gtt_send s s' ys2) S T S' T' xs0).
+      assert(forall LP LQ : list (option (sort * ltt)),
+       wfgC (gtt_send s s' ys) ->
+       projectionC (gtt_send s s' ys) p (ltt_send q LP) ->
+       subtypeC (ltt_send q (extendLis l (Some (S, T)))) (ltt_send q LP) ->
+       projectionC (gtt_send s s' ys) q (ltt_recv p LQ) ->
+       subtypeC (ltt_recv p xs0) (ltt_recv p LQ) ->
+       exists L : ltt, projectionC (gtt_send s s' ys2) p L /\ subtypeC T L).
+      {
+        intros. specialize(IHxs LP0 LQ0). apply IHxs; try easy.
+        - inversion H41. inversion H42. subst. pfold. constructor; try easy.
+          admit. (* removing 1 thing from wfgC *)
+        exists ctxG. exists SI. exists Sn.
+        - split. constructor; try easy.
+        - split; intros. apply H7. inversion H31.
+          apply ha_sendp. apply ha_sendq. 
+          apply ha_sendr with (n := Nat.succ n) (s := s0) (g := g); intros; try easy.
+        - split; intros. apply H8. inversion H31.
+          apply ha_sendp. apply ha_sendq. 
+          apply ha_sendr with (n := Nat.succ n) (s := s0) (g := g); intros; try easy.
+        - split; try easy.
+      }
+      clear IHxs. rename H15 into IHxs.
+      specialize(merge_less_recv p LQ o1 ys1 H38); intros. destruct H15.
+      specialize(merge_less_send q LP o0 ys0 H27); intros. destruct H16.
+      rename x into LQ'. rename x0 into LP'.
+      specialize(IHxs LP' LQ'); intros.
+      assert (exists L : ltt, projectionC (gtt_send s s' ys2) p L /\ subtypeC T L). 
+      {
+        apply IHxs; try easy. clear IHxs.
+        - admit. (* removing 1 thing from wfgC *)
+        - pfold. 
+          apply proj_cont with (ys := ys0); try easy. inversion H26. subst. easy.
+          apply stTrans with (l2 := (ltt_send q LP)); try easy.
+          apply more_merge_sub with (o0 := o0) (ys0 := ys0); try easy.
+        - pfold.
+          apply proj_cont with (ys := ys1); try easy. inversion H37. subst. easy.
+          apply stTrans with (l2 := (ltt_recv p LQ)); try easy.
+          apply more_merge_sub with (o0 := o1) (ys0 := ys1); try easy.
+      }
+      destruct H18. rename x into Lys. destruct H18.
+      
+      inversion H41. subst. clear H41. inversion H37. subst. clear H37.
+      inversion H42. subst. clear H42. inversion H26. subst. clear H26.
+      clear IHxs.
+      
+      destruct H10. subst.
+      - destruct H17; try easy. destruct H10. subst.
+        destruct H37. destruct H36. destruct H39. destruct H22. destruct H17. destruct H26. subst.
+        exists Lys. split; try easy.
+        pfold. 
+        pinversion H18; try easy. subst. (* participant pf, use H33 *)
+        admit.
+        subst. apply proj_cont with (ys := None :: ys3); try easy. constructor; try easy.
+        left. easy.
+        apply triv_merge2; try easy.
+        apply proj_mon.
+        destruct H26. destruct H26. destruct H26. destruct H26; try easy.
+        destruct H22. destruct H22. destruct H22. destruct H22. easy.
+        destruct H17. destruct H17. destruct H17. destruct H17. easy.
+        destruct H10. destruct H10. destruct H10. destruct H10. easy.
+        
+      - destruct H10. destruct H10. destruct H10. subst.
+        destruct H17; try easy. destruct H10. destruct H10. destruct H10. destruct H10. destruct H17.
+        inversion H10. subst. clear H10.
+        destruct H32; try easy. destruct H10. destruct H10. destruct H10. destruct H17.
+        inversion H10. subst. clear H10.
+        destruct H37; try easy. destruct H10. destruct H10. destruct H10. destruct H10. destruct H32.
+        inversion H10. subst. clear H10.
+        destruct H36; try easy. destruct H10. destruct H10. destruct H10. destruct H10. destruct H32.
+        inversion H10. subst. clear H10.
+        destruct H39; try easy. destruct H10. destruct H10. destruct H10. destruct H10. destruct H32.
+        inversion H10. subst. clear H10.
+        rename x2 into Gl. rename x3 into G. rename x4 into G'.
+        specialize(H22 p q l G G').
+        specialize(_a_29_part_helper_recv 0 (Some x5 :: ys1) x5 p LQ (eq_refl (Some x5)) H38); intros.
+        destruct H10. subst.
+        specialize(_a_29_part_helper_send 0 (Some x6 :: ys0) x6 q LP (eq_refl (Some x6)) H27); intros.
+        destruct H10. subst.
+        
+        rename x into LQs. rename x0 into LPs.
+        specialize(H22 LPs LQs S T S' T' xs0).
+        assert (exists L : ltt, projectionC G' p L /\ subtypeC T L).
+        {
+          pclearbot.
+          apply H22; try easy.
+          - admit. (* wfgC of continuation *)
+          - specialize(_a_26 (ltt_send q LP) (ltt_send q LPs) ys0 H27); intros.
+            apply stTrans with (l2 := (ltt_send q LP)); try easy.
+          - specialize(_a_26 (ltt_recv p LQ) (ltt_recv p LQs) ys1 H38); intros.
+            apply stTrans with (l2 := (ltt_recv p LQ)); try easy.
+          - destruct H35; try easy.
+          - exists ctxG. exists SI. exists Sn. 
+          split. easy.
+          - split. intros. apply H7; try easy.
+            - case_eq (eqb p s); intros.
+              assert (p = s). apply eqb_eq; try easy. subst. apply ha_sendp.
+            - case_eq (eqb p s'); intros.
+              assert (p = s'). apply eqb_eq; try easy. subst. apply ha_sendq.
+            - assert (p <> s). apply eqb_neq; try easy. 
+              assert (p <> s'). apply eqb_neq; try easy.
+              apply ha_sendr with (n := 0) (s := x1) (g := Gl); try easy.
+          - split. intros. apply H8.
+            - case_eq (eqb q s); intros.
+              assert (q = s). apply eqb_eq; try easy. subst. apply ha_sendp.
+            - case_eq (eqb q s'); intros.
+              assert (q = s'). apply eqb_eq; try easy. subst. apply ha_sendq.
+            - assert (q <> s). apply eqb_neq; try easy. 
+              assert (q <> s'). apply eqb_neq; try easy.
+              apply ha_sendr with (n := 0) (s := x1) (g := Gl); try easy.
+          - split; try easy.
+        }
+        destruct H10. destruct H10. clear H9 H22. 
+        assert (exists L, projectionC (gtt_send s s' (Some (x1, G') :: ys2)) p L). { admit. }
+        destruct H9. exists x0. rename x0 into L. split; try easy.
+        pinversion H9; try easy. subst. admit. (* doable, a bit tedious *)
+        - subst.
+        
+        
+        destruct x.
+        - exists ltt_end. split; try easy.
+          pfold. constructor; try easy.
+          admit. (* doable, a bit tedious *)
+        - 
+        
+      admit. admit.
+       
+      
+      destruct H14. destruct H15. subst. destruct ys; try easy. clear H21.
+      inversion H37. subst. clear H37. inversion H41. subst. clear H41. inversion H42. subst. clear H42.
+      destruct ys2; try easy. destruct ys1; try easy. clear H33 H20 H21.
+      inversion H26. subst. clear H26. destruct ys0; try easy. 
+      destruct H10; try easy. destruct H10. destruct H10. destruct H10.
+      inversion H10. subst. clear H10.
+      destruct H17; try easy. destruct H10. destruct H10. destruct H10. destruct H10. destruct H15.
+      inversion H10. subst. clear H10. clear H32.
+      destruct H21; try easy. destruct H10. destruct H10. destruct H10. destruct H10. destruct H15. 
+      inversion H10. subst. clear H10.
+      destruct H31; try easy. destruct H10. destruct H10. destruct H10. destruct H10. destruct H15.
+      inversion H10. subst. clear H10.
+      destruct H16; try easy. destruct H10. destruct H10. destruct H10. destruct H15. 
+      inversion H10. subst. clear H10.
+      destruct H18; try easy. destruct H10. destruct H10. destruct H10. destruct H10. destruct H18.
+      inversion H10. subst. clear H10.
+      rename x2 into Gl. rename x3 into G. rename x5 into G'.
+      specialize(H14 p q l G G').
+      
+      specialize(_a_29_part_helper_recv 0 (Some x6 :: nil) x6 p LQ (eq_refl (Some x6)) H38); intros.
+      destruct H10. subst.
+      specialize(_a_29_part_helper_send 0 (Some x4 :: nil) x4 q LP (eq_refl (Some x4)) H27); intros.
+      destruct H10. subst.
+      rename x1 into LP'. rename x0 into LQ'.
+      specialize(H14 LP' LQ' S T S' T' xs0).
+      assert (exists L : ltt, projectionC G' p L /\ subtypeC T L).
+      {
+        pclearbot.
+        apply H14; try easy.
+        - admit. (* wfgC of element in continuation *)
+        - specialize(_a_26 (ltt_send q LP) (ltt_send q LP') nil H27); intros.
+          apply stTrans with (l2 := (ltt_send q LP)); try easy.
+        - specialize(_a_26 (ltt_recv p LQ) (ltt_recv p LQ') nil H38); intros.
+          apply stTrans with (l2 := (ltt_recv p LQ)); try easy.
+        - destruct H21; try easy.
+        - exists ctxG. exists SI. exists Sn. 
+        split. easy.
+        - split. intros. apply H7; try easy.
+          - case_eq (eqb p s); intros.
+            assert (p = s). apply eqb_eq; try easy. subst. apply ha_sendp.
+          - case_eq (eqb p s'); intros.
+            assert (p = s'). apply eqb_eq; try easy. subst. apply ha_sendq.
+          - assert (p <> s). apply eqb_neq; try easy. 
+            assert (p <> s'). apply eqb_neq; try easy.
+            apply ha_sendr with (n := 0) (s := x) (g := Gl); try easy.
+        - split. intros. apply H8.
+          - case_eq (eqb q s); intros.
+            assert (q = s). apply eqb_eq; try easy. subst. apply ha_sendp.
+          - case_eq (eqb q s'); intros.
+            assert (q = s'). apply eqb_eq; try easy. subst. apply ha_sendq.
+          - assert (q <> s). apply eqb_neq; try easy. 
+            assert (q <> s'). apply eqb_neq; try easy.
+            apply ha_sendr with (n := 0) (s := x) (g := Gl); try easy.
+        - split; try easy.
+      }
+      destruct H10. destruct H10. 
+      exists x0. split; try easy. 
+      pfold.
+      destruct x0.
+      - apply proj_end; intros.
+        apply pmergeCR with (G := G') (r := p); try easy.
+        admit. (* participant pf, doable, because we have wfcG *)
+      - apply proj_cont with (ys := (Some (ltt_recv s0 l0) :: nil)); try easy.
+        constructor; try easy. right. exists x. exists G'. exists (ltt_recv s0 l0).
+        split. easy. split. easy. left. easy.
+        apply triv_merge; try easy.
+      - apply proj_cont with (ys := (Some (ltt_send s0 l0) :: nil)); try easy.
+        constructor; try easy. right. exists x. exists G'. exists (ltt_send s0 l0).
+        split. easy. split. easy. left. easy.
+        apply triv_merge; try easy.
+    apply step_mon.
+    apply proj_mon.
+    apply proj_mon.
+Admitted.
+      
